restored extraction

crypto/bignum/poly1305/Hacl.Bignum.Modulo.fst
@@ -4,24 +4,76 @@ open FStar.Mul
 open FStar.HyperStack
 open FStar.Buffer
 
+open Hacl.Bignum.Constants
 open Hacl.Bignum.Parameters
 open Hacl.Spec.Bignum.Bigint
 open Hacl.Bignum.Limb
 
 open Hacl.Spec.Bignum.Modulo
 
+#set-options "--initial_fuel 0 --max_fuel 0"
 
+inline_for_extraction let mask_2_42 : p:Hacl.Bignum.Wide.t{w p = pow2 42 - 1} =
+  assert_norm (pow2 64 = 0x10000000000000000); assert_norm(pow2 42 - 1 = 0x3ffffffffff);
+  limb_to_wide (uint64_to_limb 0x3ffffffffffuL)
+
+inline_for_extraction let mask_2_42' : p:t{v p = pow2 42 - 1} =
+  assert_norm (pow2 64 = 0x10000000000000000); assert_norm(pow2 42 - 1 = 0x3ffffffffff);
+  uint64_to_limb 0x3ffffffffffuL
+
+
+val reduce:
+  b:felem ->
+  Stack unit
+  (requires (fun h -> live h b /\ reduce_pre (as_seq h b)))
+  (ensures (fun h0 _ h1 -> live h0 b /\ reduce_pre (as_seq h0 b) /\ live h1 b /\ modifies_1 b h0 h1
+    /\ as_seq h1 b == reduce_spec (as_seq h0 b)))
 let reduce b =
+  assert_norm(pow2 4 = 16);
+  assert_norm(pow2 2 = 4);
   let b0 = b.(0ul) in
-  b.(0ul) <- (five <<^ 2ul) *^ b0
+  Math.Lemmas.modulo_lemma (v b0 * 16) (pow2 64);
+  Math.Lemmas.modulo_lemma (v b0 * 4) (pow2 64);
+  b.(0ul) <- (b0 <<^ 4ul) +^ (b0 <<^ 2ul)
 
 
+#set-options "--z3rlimit 20"
+
+val carry_top:
+  b:felem ->
+  Stack unit
+  (requires (fun h -> live h b /\ carry_top_pre (as_seq h b)))
+  (ensures (fun h0 _ h1 -> live h0 b /\ carry_top_pre (as_seq h0 b) /\ live h1 b /\ modifies_1 b h0 h1
+    /\ as_seq h1 b == carry_top_spec (as_seq h0 b)))
+let carry_top b =
+  let b2 = b.(2ul) in
+  let b0 = b.(0ul) in
+  assert_norm((1 * pow2 limb_size) % pow2 (word_size) = pow2 (limb_size));
+  assert_norm(pow2 limb_size > 1);
+  Math.Lemmas.modulo_lemma (v b2 / pow2 42) (pow2 word_size);
+  let b2_42 = b2 >>^ 42ul in
+  cut (v b2_42 = v b2 / pow2 42);
+  assert_norm(pow2 2 = 4); Math.Lemmas.modulo_lemma (v b2_42 * 4) (pow2 64);
+  b.(2ul) <- b2 &^ mask_2_42';
+  b.(0ul) <- ((b2_42 <<^ 2ul) +^ b2_42) +^ b0
+
+
+val carry_top_wide:
+  b:felem_wide ->
+  Stack unit
+    (requires (fun h -> live h b /\ carry_top_wide_pre (as_seq h b)))
+    (ensures (fun h0 _ h1 -> live h0 b /\ carry_top_wide_pre (as_seq h0 b) /\ live h1 b /\ modifies_1 b h0 h1
+      /\ as_seq h1 b == carry_top_wide_spec (as_seq h0 b)))
 let carry_top_wide b =
   let b2 = b.(2ul) in
   let b0 = b.(0ul) in
   let open Hacl.Bignum.Wide in
-  let mask = (wide_one <<^ 42ul) -^ wide_one in
-  let b2' = b2 &^ mask in
-  let b0' = b0 +^ (five *^ (wide_to_limb (b2 >>^ 42ul))) in
+  assert_norm((1 * pow2 limb_size) % pow2 (2 * word_size) = pow2 (limb_size));
+  assert_norm(pow2 limb_size > 1);
+  let b2' = b2 &^ mask_2_42 in
+  Math.Lemmas.modulo_lemma (v b2 / pow2 42) (pow2 word_size);
+  let b2_42 = wide_to_limb (b2 >>^ 42ul) in
+  assert_norm(pow2 2 = 4); Math.Lemmas.modulo_lemma (Hacl.Bignum.Limb.v b2_42 * 4) (pow2 64);
+  let b0' = b0 +^ limb_to_wide Hacl.Bignum.Limb.((b2_42 <<^ 2ul) +^ b2_42) in
   b.(2ul) <- b2';
   b.(0ul) <- b0'
